I wasn't happy with `const` polluting the global name space
if IP_Addresses gets into the afp

thy/Iptables_Semantics/Routing/IpRoute_Parser.ml
@@ -50,7 +50,7 @@ local
   val parser_dev = (Scan.this_string "dev" -- parser_whitespace |-- parser_interface)
     >> (fn dev => fn pk => @{term "routing_action_oiface_update :: string \<Rightarrow> routing_rule \<Rightarrow> routing_rule"} $ dev $ pk)
   val parser_metric = (Scan.this_string "metric" -- parser_whitespace |-- Scan.many1 Symbol.is_ascii_digit)
-    >> (fn metric => fn pk => @{term "metric_update :: (nat \<Rightarrow> nat) \<Rightarrow> routing_rule \<Rightarrow> routing_rule"} $ (@{term "const :: nat \<Rightarrow> nat \<Rightarrow> nat"} $ (mk_nat 65535 (extract_int metric))) $ pk)
+    >> (fn metric => fn pk => @{term "metric_update :: (nat \<Rightarrow> nat) \<Rightarrow> routing_rule \<Rightarrow> routing_rule"} $ (@{term "(\<lambda> x _. x) :: nat \<Rightarrow> nat \<Rightarrow> nat"} $ (mk_nat 65535 (extract_int metric))) $ pk)
   (* these are going to be ignored anyway\<dots>(?) *)
   val parser_scope = (Scan.this_string "scope" -- parser_whitespace |-- (
     Scan.this_string "host" || Scan.this_string "link" || Scan.this_string "global" || (Scan.many1 Symbol.is_ascii_digit >> implode)))
