thy/Iptables_Semantics/Routing/IpRoute_Parser.thy
@@ -4,10 +4,21 @@ keywords "parse_ip_route" :: thy_decl
 begin
 
 definition "empty_rr_hlp pm = routing_rule.make pm default_metric (routing_action.make '''' None)"
+
 lemma empty_rr_hlp_alt: "empty_rr_hlp pm = \<lparr> routing_match = pm, metric = 0, routing_action = \<lparr>output_iface = [], next_hop = None\<rparr>\<rparr>"
 unfolding empty_rr_hlp_def routing_rule.defs default_metric_def routing_action.defs ..
-definition "routing_action_next_hop_update h pk = routing_action_update (next_hop_update (const (Some h))) (pk::routing_rule)"
-definition "routing_action_oiface_update h pk = routing_action_update (output_iface_update (const h)) (pk::routing_rule)"
+
+definition routing_action_next_hop_update :: "32 word \<Rightarrow> routing_rule \<Rightarrow> routing_rule"
+  where
+  "routing_action_next_hop_update h pk = pk\<lparr> routing_action := (routing_action pk)\<lparr> next_hop := Some h\<rparr> \<rparr>"
+lemma "routing_action_next_hop_update h pk = routing_action_update (next_hop_update (\<lambda>_. (Some h))) (pk::routing_rule)"
+  by(simp add: routing_action_next_hop_update_def)
+
+definition routing_action_oiface_update :: "string \<Rightarrow> routing_rule \<Rightarrow> routing_rule"
+  where
+  "routing_action_oiface_update h pk = routing_action_update (output_iface_update (\<lambda>_. h)) (pk::routing_rule)"
+lemma "routing_action_oiface_update h pk = pk\<lparr> routing_action := (routing_action pk)\<lparr> output_iface :=  h\<rparr> \<rparr>"
+  by(simp add: routing_action_oiface_update_def)
 
 (* Hide all the ugly ml in a file with the right extension *)
 term PrefixMatch
@@ -19,7 +30,15 @@ ML\<open>
   (Parse.binding --| @{keyword "="} -- Parse.string >> register_ip_route)
 \<close>
 
-parse_ip_route "rtbl_parser_test1" = "ip-route-ex"  value rtbl_parser_test1
+parse_ip_route "rtbl_parser_test1" = "ip-route-ex"
+
+lemma "rtbl_parser_test1 =
+  [\<lparr>routing_match = PrefixMatch 0xFFFFFF00 32, metric = 0, routing_action = \<lparr>output_iface = ''tun0'', next_hop = None\<rparr>\<rparr>,
+  \<lparr>routing_match = PrefixMatch 0xA0D2AA0 28, metric = 303, routing_action = \<lparr>output_iface = ''ewlan'', next_hop = None\<rparr>\<rparr>,
+  \<lparr>routing_match = PrefixMatch 0xA0D2500 24, metric = 0, routing_action = \<lparr>output_iface = ''tun0'', next_hop = Some 0xFFFFFF00\<rparr>\<rparr>,
+  \<lparr>routing_match = PrefixMatch 0xA0D2C00 24, metric = 0, routing_action = \<lparr>output_iface = ''tun0'', next_hop = Some 0xFFFFFF00\<rparr>\<rparr>,
+  \<lparr>routing_match = PrefixMatch 0 0, metric = 303, routing_action = \<lparr>output_iface = ''ewlan'', next_hop = Some 0xA0D2AA1\<rparr>\<rparr>]"
+by eval
 
 
 end
